Contracts/Common.lean
@@ -71,8 +71,12 @@ def ecrecover (hash v r sigS : Uint256) : Contract Address := fun state =>
 def calldatacopy (_destOffset _sourceOffset _size : Uint256) : Contract Unit := pure ()
 def returndataCopy (_destOffset _sourceOffset _size : Uint256) : Contract Unit := pure ()
 def revertReturndata : Contract Unit := pure ()
+def arrayLength {α : Type} (values : Array α) : Uint256 := values.size
+def arrayElement {α : Type} [Inhabited α] (values : Array α) (index : Uint256) : α :=
+  values.getD (index : Nat) default
+def returnArray {α : Type} (values : Array α) : Contract (Array α) := pure values
 def returnValues (_values : List Uint256) : Contract Unit := pure ()
-def returnBytes {α : Type} [Inhabited α] (_value : α) : Contract α := pure default
+def returnBytes {α : Type} (value : α) : Contract α := pure value
 def returnStorageWords (_slots : Array Uint256) : Contract (Array Uint256) := pure #[]
 def mstore (_offset _value : Uint256) : Contract Unit := pure ()
 def getMappingWord (_slot : StorageSlot (Uint256 → Uint256)) (_key _wordOffset : Uint256) :
